refactor

runtime.c
@@ -1,0 +1,7 @@
+#include <lean/lean.h>
+
+LEAN_EXPORT LEAN_NORETURN lean_object *
+tmeta_panic_thunk(lean_object *message, lean_object *unit) {
+    (void)unit;
+    lean_internal_panic(lean_string_cstr(message));
+}
