TMeta/Elab/OpTransform.lean
@@ -1,0 +1,141 @@
+module
+
+public import Lean.Meta.Basic
+
+open Lean Meta
+
+namespace TMeta.Elab.OpTransform
+
+/--
+Decomposes an application into its head and its application nodes, ordered
+from outermost to innermost.
+-/
+@[inline]
+def withAppSpine (e : Expr) (k : Expr → Array Expr → α) : α :=
+  go e #[]
+where
+  go (e : Expr) (apps : Array Expr) : α :=
+    match e with
+    | .app fn _ => go fn (apps.push e)
+    | fn => k fn apps
+
+@[inline]
+private unsafe def mapUnderBinders!Impl [Monad m] [MonadLiftT MetaM m]
+    (expr : Expr) (fvars : Array Expr)
+    (f : Expr → m Expr) (k : Expr → Expr → m α) : m α := do
+  let inst := expr.instantiateRev fvars
+  let result ← f inst
+  if ptrEq inst result then
+    k inst expr
+  else
+    k inst (← result.abstractM fvars)
+
+/--
+Instantiates an expression with `fvars`, applies `f` to it, and abstracts the
+result again. Passes the instantiated expression and the abstracted result to
+`k`. If `f` returns a pointer-equal result, the runtime implementation also
+returns a pointer-equal abstracted result.
+-/
+@[implemented_by mapUnderBinders!Impl]
+def mapUnderBinders! [Monad m] [MonadLiftT MetaM m]
+    (expr : Expr) (fvars : Array Expr)
+    (f : Expr → m Expr) (k : Expr → Expr → m α) : m α := do
+  let inst := expr.instantiateRev fvars
+  k inst (← (← f inst).abstractM fvars)
+
+public section
+
+inductive OpAppTransform (m : Type → Type) where
+  | default
+  | skip (n : Nat)
+  | transform {n : Nat} (onOpApp : (fn : Expr) → (args : Vector Expr n) → m Expr)
+  deriving Inhabited
+
+variable [Monad m] [MonadError m] [MonadLiftT MetaM m] [MonadControlT MetaM m]
+
+variable (getOpAppTransform : Name → OpAppTransform m)
+
+mutual
+
+partial def transform (e : Expr) : m Expr := do
+  match e with
+  | .app .. =>
+      transformApp e
+  | .lam .. | .letE .. =>
+      transformLambdaLet e #[]
+  | .forallE .. =>
+      transformForall e #[]
+  | .mdata _ body =>
+      return e.updateMData! (← transform body)
+  | .proj _ _ body =>
+      return e.updateProj! (← transform body)
+  | .sort .. | .const .. | .fvar .. | .mvar .. | .lit .. =>
+      return e
+  | .bvar _ =>
+      throwError "unexpected loose bound variable"
+
+partial def transformApp (e : Expr) : m Expr :=
+  withAppSpine e fun fn apps =>
+    if let fn'@(.const name _) := fn.cleanupAnnotations then
+      match getOpAppTransform name with
+      | .default =>
+          transformAppDefault fn apps
+      | .skip n =>
+          if hu : n ≤ apps.size then do
+            let fn := if hl : n = 0 then fn else apps[apps.size - n]
+            transformAppArgs fn apps (apps.size - n)
+          else
+            throwError "operator '{name}' expected at least {n} arguments, got {apps.size}"
+      | .transform onOpApp (n := n) =>
+          let args := apps.map (·.appArg!)
+          if h : n ≤ args.size then do
+            let fn ← onOpApp fn' (.ofFn fun i => args[args.size - 1 - i])
+            args.foldrM (init := fn) (start := args.size - n) fun app fn => do
+              return .app fn (← transform app)
+          else
+            throwError "operator '{name}' expected at least {n} arguments, got {apps.size}"
+    else
+      transformAppDefault fn apps
+
+partial def transformAppDefault (fn : Expr) (apps : Array Expr) : m Expr := do
+  let fn ← transform fn
+  transformAppArgs fn apps apps.size
+
+partial def transformAppArgs (fn : Expr) (apps : Array Expr) (size : Nat) : m Expr :=
+  apps.foldrM (init := fn) (start := size) fun app fn => do
+    let arg ← transform app.appArg!
+    return app.updateApp! fn arg
+
+partial def transformLambdaLet (e : Expr) (fvars : Array Expr) : m Expr := do
+  match e with
+  | .lam name domain body bi =>
+      mapUnderBinders! domain fvars transform fun instDomain domain =>
+        withLocalDecl name bi instDomain fun x => do
+          let body ← transformLambdaLet body (fvars.push x)
+          return e.updateLambdaE! domain body
+  | .letE name domain value body nondep =>
+      mapUnderBinders! domain fvars transform fun instDomain domain =>
+        mapUnderBinders! value fvars transform fun instValue value =>
+          withLetDecl name instDomain instValue (nondep := nondep) fun x => do
+            let body ← transformLambdaLet body (fvars.push x)
+            return e.updateLetE! domain value body
+  | body =>
+      mapUnderBinders! body fvars transform fun _ body =>
+        return body
+
+partial def transformForall (e : Expr) (fvars : Array Expr) : m Expr := do
+  match e with
+  | .forallE name domain body bi =>
+      mapUnderBinders! domain fvars transform fun instDomain domain =>
+        withLocalDecl name bi instDomain fun x => do
+          let body ← transformForall body (fvars.push x)
+          return e.updateForallE! domain body
+  | body =>
+      mapUnderBinders! body fvars transform fun _ body =>
+        return body
+
+end
+
+end
+
+end TMeta.Elab.OpTransform
